src/tls/TLSInfo.fst
@@ -17,7 +17,6 @@ open TLSConstants
 
 module CC = CoreCrypto
 module MM = FStar.Monotonic.Map
-module MR = FStar.Monotonic.RRef
 
 let default_cipherSuites = [
   TLS_AES_128_GCM_SHA256;
@@ -517,7 +516,7 @@ let safety_table: s_table =
 type registered (i:pre_index) =
   (if Flags.ideal_KEF then
     let log: i_safety_log = safety_table in
-    MR.witnessed (MM.defined log i)
+    witnessed (MM.defined log i)
   else True)
 
 type valid (i:pre_index) =
@@ -568,13 +567,13 @@ type index = i:pre_index{valid i}
 type honest (i:index) =
   (if Flags.ideal_KEF then
     let log : i_safety_log = safety_table in
-    MR.witnessed (MM.contains log i true)
+    witnessed (MM.contains log i true)
   else False)
 
 type dishonest (i:index) =
   (if Flags.ideal_KEF then
     let log : i_safety_log = safety_table in
-    MR.witnessed (MM.contains log i false)
+    witnessed (MM.contains log i false)
   else True)
 
 // type esId = i:pre_esId{valid (I_ES i)}
